feat: add `uset`

Batteries/Data/DArray.lean
@@ -49,6 +49,9 @@ private unsafe def ugetImpl (a : DArray n α) (i : USize) (h : i.toNat < n) : α
 private unsafe def setImpl (a : DArray n α) (i) (v : α i) : DArray n α :=
   unsafeCast <| a.data.set ⟨i.val, lcProof⟩ <| unsafeCast v
 
+private unsafe def usetImpl (a : DArray n α) (i : USize) (h : i.toNat < n) (v : α ⟨i.toNat, h⟩) :
+    DArray n α := unsafeCast <| a.data.uset i (unsafeCast v) lcProof
+
 private unsafe def copyImpl (a : DArray n α) : DArray n α :=
   unsafeCast <| a.data.extract 0 n
 
@@ -84,6 +87,14 @@ attribute [implemented_by casesOnImpl] DArray.casesOn
 protected def set (a : DArray n α) (i : Fin n) (v : α i) : DArray n α :=
   mk fun j => if h : i = j then h ▸ v else a.get j
 
+/--
+Sets the `DArray` item at index `i : USize`.
+Slightly faster than `set` and `O(1)` if exclusive else `O(n)`.
+-/
+@[implemented_by usetImpl]
+protected def uset (a : DArray n α) (i : USize) (h : i.toNat < n) (v : α ⟨i.toNat, h⟩) :=
+  a.set ⟨i.toNat, h⟩ v
+
 @[simp, inherit_doc DArray.set]
 protected abbrev setN (a : DArray n α) (i) (h : i < n := by get_elem_tactic) (v : α ⟨i, h⟩) :=
   a.set ⟨i, h⟩ v
@@ -103,10 +114,6 @@ theorem set_mk {α : Fin n → Type _} {init : (i : Fin n) → α i} (i : Fin n)
     DArray.set (.mk init) i v = .mk fun j => if h : i = j then h ▸ v else init j := rfl
 
 @[simp]
-theorem uget_eq_get (a : DArray n α) (i : USize) (h : i.toNat < n) :
-    a.uget i h = a.get ⟨i.toNat, h⟩ := rfl
-
-@[simp]
 theorem get_set (a : DArray n α) (i : Fin n) (v : α i) : (a.set i v).get i = v := by
   simp only [DArray.get, DArray.set, dif_pos]
 
@@ -120,6 +127,14 @@ theorem set_set (a : DArray n α) (i : Fin n) (v w : α i) : (a.set i v).set i w
     rw [← h, get_set, get_set]
   else
     rw [get_set_ne _ _ h, get_set_ne _ _ h, get_set_ne _ _ h]
+
+@[simp]
+theorem uget_eq_get (a : DArray n α) (i : USize) (h : i.toNat < n) :
+    a.uget i h = a.get ⟨i.toNat, h⟩ := rfl
+
+@[simp]
+theorem uset_eq_set (a : DArray n α) (i : USize) (h : i.toNat < n) (v : α ⟨i.toNat, h⟩) :
+    a.uset i h v = a.set ⟨i.toNat, h⟩ v := rfl
 
 @[simp]
 theorem copy_eq (a : DArray n α) : a.copy = a := rfl
